theories/LogicalRelation/SimpleArr.v
@@ -1,6 +1,6 @@
 From LogRel.AutoSubst Require Import core unscoped Ast Extra.
-From LogRel Require Import Notations Utils BasicAst Context NormalForms Weakening GenericTyping LogicalRelation DeclarativeInstance.
-From LogRel.LogicalRelation Require Import Induction Irrelevance Weakening Neutral Escape Reflexivity NormalRed Reduction Transitivity Application.
+From LogRel Require Import Notations Utils BasicAst LContexts Context NormalForms Weakening GenericTyping LogicalRelation Monad.
+From LogRel.LogicalRelation Require Import Induction Irrelevance Weakening Neutral Escape Reflexivity NormalRed Reduction Monotonicity Transitivity Application.
 
 Set Universe Polymorphism.
 Set Printing Primitive Projection Parameters.
@@ -8,88 +8,310 @@ Set Printing Primitive Projection Parameters.
 Section SimpleArrow.
   Context `{GenericTypingProperties}.
   
-  Lemma ArrRedTy0 {Γ l A B} : [Γ ||-<l> A] -> [Γ ||-<l> B] -> [Γ ||-Π<l> arr A B].
+  Lemma shiftPolyRed {wl Γ l A B} :
+    [Γ ||-<l> A]< wl > ->
+    [Γ ||-<l> B]< wl > ->
+    PolyRed wl Γ l A B⟨↑⟩.
+  Proof.
+    intros; escape; unshelve econstructor.
+    - intros; eapply wk ; eauto.
+      now eapply Ltrans.
+    - intros.
+      now econstructor.
+    - intros; bsimpl; rewrite <- rinstInst'_term; eapply wk.
+      + now eapply wfc_Ltrans.
+      + eapply Ltrans ; [ | eassumption].
+        eapply wfLCon_le_trans ; eauto.
+    - intros ; now econstructor.
+    - now escape.
+    - renToWk; eapply wft_wk; gen_typing.
+    - intros; irrelevance0.
+      2: replace (subst_term _ _) with B⟨ρ⟩.
+      2: eapply wkEq, reflLRTyEq.
+      all: bsimpl; now rewrite rinstInst'_term.
+      Unshelve. 1: tea.
+      + now eapply wfc_Ltrans.
+      + eapply Ltrans ; [ | eassumption].
+        eapply wfLCon_le_trans ; eauto.
+  Qed.
+
+
+  Lemma ArrRedTy0 {wl Γ l A B} :
+    [Γ ||-<l> A]< wl > ->
+    [Γ ||-<l> B]< wl > ->
+    [Γ ||-Π<l> arr A B]< wl >.
   Proof.
     intros RA RB; escape.
     unshelve econstructor; [exact A| exact B⟨↑⟩|..]; tea.
-    - intros; now eapply wk.
-    - cbn; intros.
-      bsimpl; rewrite <- rinstInst'_term.
-      now eapply wk.
     - eapply redtywf_refl.
       now eapply wft_simple_arr.
-    - renToWk; eapply wft_wk; gen_typing.
+    - now unshelve eapply escapeEq, reflLRTyEq.
     - eapply convty_simple_arr; tea.
-      all: now unshelve eapply escapeEq, LRTyEqRefl_.
-    - intros; irrelevance0.
-      2: replace (subst_term _ _) with B⟨ρ⟩.      
-      2: eapply wkEq, LRTyEqRefl_.
-      all: bsimpl; now rewrite rinstInst'_term.
-      Unshelve. all: tea.
+      all: now unshelve eapply escapeEq, reflLRTyEq.
+    - now eapply shiftPolyRed.
   Qed.
 
-  Lemma ArrRedTy {Γ l A B} : [Γ ||-<l> A] -> [Γ ||-<l> B] -> [Γ ||-<l> arr A B].
+  Lemma ArrRedTy {wl Γ l A B} :
+    [Γ ||-<l> A]< wl > ->
+    [Γ ||-<l> B]< wl > ->
+    [Γ ||-<l> arr A B]< wl >.
   Proof. intros; eapply LRPi'; now eapply ArrRedTy0. Qed.
 
-  Lemma idred {Γ l A} (RA : [Γ ||-<l> A]) :
-    [Γ ||-<l> idterm A : arr A A | ArrRedTy RA RA].
+  Lemma WArrRedTy {wl Γ l A B} :
+    W[Γ ||-<l> A]< wl > ->
+    W[Γ ||-<l> B]< wl > ->
+    W[Γ ||-<l> arr A B]< wl >.
   Proof.
+    intros [WTA WRedA] [WTB WRedB].
+    exists (DTree_fusion _ WTA WTB).
+    intros ; eapply ArrRedTy.
+    - now eapply WRedA, over_tree_fusion_l.
+    - now eapply WRedB, over_tree_fusion_r.
+  Qed.
+
+  Lemma shiftPolyRedEq {wl Γ l A A' B B'}
+    (RA : [Γ ||-<l> A]< wl >)
+    (RB : [Γ ||-<l> B]< wl >)
+    (PAB : PolyRed wl Γ l A B⟨↑⟩) :
+    [Γ ||-<l> A ≅ A' | RA]< wl > ->
+    [Γ ||-<l> B ≅ B' | RB]< wl > ->
+    PolyRedEq PAB A' B'⟨↑⟩.
+  Proof.
+    intros; escape; unshelve econstructor.
+    - intros ; now econstructor.
+    - intros; irrelevanceRefl; eapply wkEq.
+      unshelve eapply (Eq_Ltrans f) ; eassumption.
+    - intros; irrelevance0; rewrite shift_subst_scons; [reflexivity|].
+      eapply wkEq, (Eq_Ltrans (wfLCon_le_trans _ f)) ; eassumption.
+      Unshelve. all: eauto.
+      now eapply wfc_Ltrans.
+  Qed.
+
+  Lemma arrRedCong0 {wl Γ l A A' B B'}
+    (RA : [Γ ||-<l> A]< wl >)
+    (RB : [Γ ||-<l> B]< wl >)
+    (tyA' : [Γ |- A']< wl >)
+    (tyB' : [Γ |- B']< wl >)
+    (RAB : [Γ ||-Π<l> arr A B]< wl >) :
+    [Γ ||-<l> A ≅ A' | RA]< wl > ->
+    [Γ ||-<l> B ≅ B' | RB]< wl > ->
+    [Γ ||-Π arr A B ≅ arr A' B' | normRedΠ0 RAB]< wl >.
+  Proof.
+    intros RAA' RBB'; escape.
+    unshelve econstructor; cycle 2.
+    + eapply redtywf_refl; now eapply wft_simple_arr.
+    + now cbn.
+    + now eapply convty_simple_arr.
+    + now eapply shiftPolyRedEq.
+  Qed.
+    
+  Lemma arrRedCong {wl Γ l A A' B B'}
+    (RA : [Γ ||-<l> A]< wl >) (RB : [Γ ||-<l> B]< wl >)
+    (tyA' : [Γ |- A']< wl >) (tyB' : [Γ |- B']< wl >) :
+    [Γ ||-<l> A ≅ A' | RA]< wl > ->
+    [Γ ||-<l> B ≅ B' | RB]< wl > ->
+    [Γ ||-<l> arr A B ≅ arr A' B' | normRedΠ (ArrRedTy RA RB)]< wl >.
+  Proof.
+    intros; now eapply arrRedCong0.
+  Qed.
+
+  Lemma arrRedCong' {wl Γ l A A' B B'}
+    (RA : [Γ ||-<l> A]< wl >) (RB : [Γ ||-<l> B]< wl >)
+    (tyA' : [Γ |- A']< wl >) (tyB' : [Γ |- B']< wl >)
+    (RAB : [Γ ||-<l> arr A B]< wl >) :
+    [Γ ||-<l> A ≅ A' | RA]< wl > ->
+    [Γ ||-<l> B ≅ B' | RB]< wl > ->
+    [Γ ||-<l> arr A B ≅ arr A' B' | RAB]< wl >.
+  Proof.
+    intros; irrelevanceRefl; now eapply arrRedCong.
+  Qed.
+
+  Lemma WarrRedCong' {wl Γ l A A' B B'}
+    (RA : W[Γ ||-<l> A]< wl >) (RB : W[Γ ||-<l> B]< wl >)
+    (tyA' : [Γ |- A']< wl >) (tyB' : [Γ |- B']< wl >)
+    (RAB : W[Γ ||-<l> arr A B]< wl >) :
+    W[Γ ||-<l> A ≅ A' | RA]< wl > ->
+    W[Γ ||-<l> B ≅ B' | RB]< wl > ->
+    W[Γ ||-<l> arr A B ≅ arr A' B' | RAB]< wl >.
+  Proof.
+    intros [WTAA WEqA] [WTBB WEqB].
+    exists (DTree_fusion _ (DTree_fusion _ (WT _ RA) (WT _ RB))
+              (DTree_fusion _ WTAA WTBB)).
+    intros wl' Hover hover'.
+    pose proof (f := over_tree_le Hover).
+    eapply arrRedCong'.
+    1,2: now eapply wft_Ltrans.
+    - unshelve eapply WEqA.
+      + now do 2 (eapply over_tree_fusion_l).
+      + now eapply over_tree_fusion_l, over_tree_fusion_r.
+    - unshelve eapply WEqB.
+      + now eapply over_tree_fusion_r, over_tree_fusion_l.
+      + now do 2 (eapply over_tree_fusion_r).
+  Qed.
+
+  Lemma polyRedArrExt {wl Γ l A B C} :
+    PolyRed wl Γ l A B -> PolyRed wl Γ l A C -> PolyRed wl Γ l A (arr B C).
+  Proof.
+    intros [tyA tyB RA RTree RB RBExtTree RBext] [_ tyC RA' RTree' RC RCExtTree RCext].
+    unshelve econstructor.
+    6: now eapply wft_simple_arr.
+    1,5: eassumption.
+    + intros ; eapply DTree_fusion.
+       * unshelve eapply RTree.
+         3-5: eassumption.
+         2: irrelevance0 ; [ reflexivity | eassumption].
+       * unshelve eapply RTree'.
+         3-5: eassumption.
+         2: irrelevance0 ; [ reflexivity | eassumption].
+    + intros; rewrite subst_arr; refold.
+      apply ArrRedTy; [eapply RB| eapply RC].
+      cbn in *.
+      * now eapply over_tree_fusion_l.
+      * now eapply over_tree_fusion_r.
+    + intros ; eapply DTree_fusion.
+       * unshelve eapply (RBExtTree _ _ a b).
+         2-4: eassumption.
+         1-3 : irrelevance0 ; [ reflexivity | eassumption].
+       * unshelve eapply (RCExtTree _ _ a b).
+         2-4: eassumption.
+         1-3: irrelevance0 ; [reflexivity | eassumption].
+    + intros.
+      irrelevance0; rewrite subst_arr; [refold; reflexivity|]; refold.
+      unshelve eapply arrRedCong.
+      3,4: eapply escapeConv ; first [eapply RBext | eapply RCext] ; cycle 1.
+      7,8: first [eapply RBext| eapply RCext].
+      all: cbn in *.
+      Unshelve.
+      all: try (eapply over_tree_fusion_l ; eassumption).
+      all: try (eapply over_tree_fusion_r ; eassumption).
+  Qed.
+
+  Lemma polyRedEqArrExt {wl Γ l A A' B B' C C'}
+    (PAB : PolyRed wl Γ l A B) (PAC : PolyRed wl Γ l A C) 
+    (PAB' : PolyRed wl Γ l A' B') (PAC' : PolyRed wl Γ l A' C') 
+    (PABC : PolyRed wl Γ l A (arr B C))
+    (PABeq : PolyRedEq PAB A' B')
+    (PACeq : PolyRedEq PAC A' C')
+    : PolyRedEq PABC A' (arr B' C').
+  Proof.
+    econstructor.
+    + intros; irrelevanceRefl; now unshelve eapply (PolyRedEq.shpRed PABeq).
+    + intros; irrelevance0; rewrite subst_arr; refold; [reflexivity|].
+      pose proof (f' := over_tree_le Ho).
+      apply arrRedCong.
+      * eapply escapeConv.
+        unshelve eapply (PolyRedEq.posRed PABeq) ; cycle 1 ; try eassumption.
+        -- now irrelevance0.
+        -- do 3 (eapply over_tree_fusion_l) ; exact Ho' .
+        -- eapply over_tree_fusion_r ; do 2 (eapply over_tree_fusion_l) ; exact Ho'.
+      * eapply escape; unshelve eapply (PolyRed.posRed).
+        5: exact f.
+        4: eapply LRTmRedConv; tea.
+        4: irrelevanceRefl; unshelve eapply (PolyRedEq.shpRed PABeq).
+        1,2,3,4: eassumption.
+        eapply over_tree_fusion_r, over_tree_fusion_l ; exact Ho'.
+      * unshelve eapply (PolyRedEq.posRed PABeq).
+        2,3: eassumption.
+        1: now irrelevanceRefl.
+        all: cbn in *.
+        1: now do 3 (eapply over_tree_fusion_l).
+        now eapply over_tree_fusion_r ; do 2 (eapply over_tree_fusion_l).
+      * unshelve eapply (PolyRedEq.posRed PACeq).
+        2,3: eassumption.
+        1: now irrelevanceRefl.
+        all: cbn in *.
+        eapply over_tree_fusion_l, over_tree_fusion_r ; exact Ho'.
+        do 2 (eapply over_tree_fusion_r) ; exact Ho'.
+  Qed.
+
+  Lemma idred {wl Γ l A} (RA : [Γ ||-<l> A]< wl >) :
+    [Γ ||-<l> idterm A : arr A A | ArrRedTy RA RA]< wl >.
+  Proof.
+    eassert [_ | Γ,, A ||- tRel 0 : A⟨_⟩]< wl > as hrel.
+    {
+      eapply var0.
+      1: reflexivity.
+      now escape.
+    }
+    Unshelve.
+    all: cycle -1.
+    { 
+      erewrite <- wk1_ren_on.
+      eapply wk ; tea.
+      escape.
+      gen_typing.
+    }
+    eapply reflLRTmEq in hrel.
     normRedΠ ΠAA.
-    pose proof (LRTyEqRefl_ RA).
+    pose proof (reflLRTyEq RA).
     escape.
-    assert (h : forall Δ a (ρ : Δ ≤ Γ) (wfΔ : [|- Δ]) RA (ha : [Δ ||-<l> a : A⟨ρ⟩ | RA]),
-      [Δ ||-<l> tApp (idterm A)⟨ρ⟩ a : A⟨ρ⟩| RA] ×
-      [Δ ||-<l> tApp (idterm A)⟨ρ⟩ a ≅ a : A⟨ρ⟩| RA]
+    assert (h : forall Δ wl' a (ρ : Δ ≤ Γ) (f : wl' ≤ε wl)
+                       (wfΔ : [|- Δ]< wl' >) RA
+                       (ha : [Δ ||-<l> a : A⟨ρ⟩ | RA]< wl' >),
+      [Δ ||-<l> tApp (idterm A)⟨ρ⟩ a : A⟨ρ⟩| RA]< wl' > ×
+      [Δ ||-<l> tApp (idterm A)⟨ρ⟩ a ≅ a : A⟨ρ⟩| RA]< wl' >
     ).
     1:{
       intros; cbn; escape.
-      assert [Δ |- A⟨ρ⟩] by now eapply wft_wk.
-      assert [Δ |- A⟨ρ⟩ ≅ A⟨ρ⟩] by now eapply convty_wk.
+      assert [Δ |- A⟨ρ⟩]< wl' > by (eapply wft_wk ; eauto ; now eapply wft_Ltrans).
+      assert [Δ |- A⟨ρ⟩ ≅ A⟨ρ⟩]< wl' >
+        by (eapply convty_wk ; eauto ; now eapply convty_Ltrans).
       eapply redSubstTerm; tea.
       now eapply redtm_id_beta.
     }
-    econstructor; cbn.
-    - eapply redtmwf_refl.
-      now eapply ty_id.
-    - constructor.
-    - apply tm_nf_lam.
-      + eapply reifyType, RA.
-      + apply tm_ne_nf, tm_ne_rel.
-        gen_typing.
-    - now eapply convtm_id.
+    unshelve econstructor; cbn.
+    4: eapply redtmwf_refl; now eapply ty_id.
+    - intros ; now econstructor.
+    - intros ; now econstructor.
+    - eapply convtm_id; tea.
+      eapply wfc_wft; now escape.
+    - unshelve econstructor 1.
+      + intros ; now econstructor.
+      + intros; cbn; apply reflLRTyEq.
+      + intros; cbn.
+        irrelevance0; [|eapply (Tm_Ltrans Ho') ; exact ha].
+        cbn; bsimpl; now rewrite rinstInst'_term.
     - intros; cbn; irrelevance0.
-      2: now eapply h.
-      bsimpl; now rewrite rinstInst'_term.
+      2: eapply h ; eauto.
+      2: now eapply wfLCon_le_trans.
+      2: now eapply wfc_Ltrans.
+      + bsimpl; now rewrite rinstInst'_term.
+      + now eapply (Tm_Ltrans Ho').
     - intros ; cbn; irrelevance0; cycle 1.
       1: eapply transEqTerm;[|eapply transEqTerm].
-      + now eapply h.
-      + eassumption.
-      + eapply LRTmEqSym. now eapply h.
+      + eapply h.
+        * now eapply wfLCon_le_trans.
+        * now eapply wfc_Ltrans.
+        * now eapply (Tm_Ltrans Hoa).
+      + eapply (TmEq_Ltrans Hoa) ; eassumption.
+      + eapply (TmEq_Ltrans Hoa),LRTmEqSym ; now eapply h.
       + bsimpl; now rewrite rinstInst'_term.
   Qed.
 
   Section SimpleAppTerm.
-    Context {Γ t u F G l}
-      {RF : [Γ ||-<l> F]}
-      (RG : [Γ ||-<l> G])
-      (hΠ := normRedΠ0 (ArrRedTy0 RF RG))
-      (Rt : [Γ ||-<l> t : arr F G | LRPi' hΠ])
-      (Ru : [Γ ||-<l> u : F | RF]).
+    Context {wl Γ t u F G l}
+      {RF : [Γ ||-<l> F]< wl >}
+      (RG : [Γ ||-<l> G]< wl >)
+      (hΠ := normRedΠ (ArrRedTy RF RG))
+      (Rt : [Γ ||-<l> t : arr F G | hΠ]< wl >)
+      (Ru : [Γ ||-<l> u : F | RF]< wl >)
+      (WRG := Build_WLogRel l wl Γ G (leaf _)
+                (fun wl Hover => Ltrans (over_tree_le Hover) RG)).
 
-    Lemma simple_app_id : [Γ ||-<l> tApp (PiRedTm.nf Rt) u : G | RG ].
+    Lemma simple_app_id : W[Γ ||-<l> tApp (PiRedTm.nf Rt) u : G | WRG ]< wl >.
     Proof.
-      irrelevance0.
-      2: now eapply app_id.
-      now bsimpl.
-      Unshelve. 1: tea.
-      now bsimpl.
+      unshelve eapply WLRTmRedIrrelevant'.
+      5: eapply app_id.
+      1: tea.
+      1,2: now bsimpl.
+      eassumption.
     Qed.
 
     Lemma simple_appTerm0 :
-        [Γ ||-<l> tApp t u : G | RG]
-        × [Γ ||-<l> tApp t u ≅ tApp (PiRedTm.nf Rt) u : G | RG].
+        W[Γ ||-<l> tApp t u : G | WRG]< wl >
+        × W[Γ ||-<l> tApp t u ≅ tApp (PiRedTm.nf Rt) u : G | WRG]< wl >.
     Proof.
-      irrelevance0.
+      eapply WLRTmTmEqIrrelevant'.
       2: now eapply appTerm0.
       now bsimpl.
       Unshelve. 1: tea.
@@ -98,135 +320,252 @@ Section SimpleArrow.
 
   End SimpleAppTerm.
 
-  Lemma simple_appTerm {Γ t u F G l}
-    {RF : [Γ ||-<l> F]}
-    (RG : [Γ ||-<l> G]) 
-    (RΠ : [Γ ||-<l> arr F G])
-    (Rt : [Γ ||-<l> t : arr F G | RΠ])
-    (Ru : [Γ ||-<l> u : F | RF]) :
-    [Γ ||-<l> tApp t u : G| RG].
-  Proof.  
-    unshelve eapply simple_appTerm0.
-    3: irrelevance.
-    all: tea.
-  Qed.
-
-
-  Lemma simple_appcongTerm {Γ t t' u u' F G l}
-    {RF : [Γ ||-<l> F]}
-    (RG : [Γ ||-<l> G])
-    (RΠ : [Γ ||-<l> arr F G]) 
-    (Rtt' : [Γ ||-<l> t ≅ t' : _ | RΠ])
-    (Ru : [Γ ||-<l> u : F | RF])
-    (Ru' : [Γ ||-<l> u' : F | RF])
-    (Ruu' : [Γ ||-<l> u ≅ u' : F | RF ]) :
-      [Γ ||-<l> tApp t u ≅ tApp t' u' : G | RG].
+  Lemma simple_appTerm {wl Γ t u F G l}
+    {RF : [Γ ||-<l> F]< wl >}
+    (RG : [Γ ||-<l> G]< wl >) 
+    (RΠ : [Γ ||-<l> arr F G]< wl >)
+    (Rt : [Γ ||-<l> t : arr F G | RΠ]< wl >)
+    (Ru : [Γ ||-<l> u : F | RF]< wl >) :
+    W[Γ ||-<l> tApp t u : G| (LogtoW RG)]< wl >.
   Proof.
-    irrelevance0.
-    2: eapply appcongTerm.
-    2-5: tea.
-    now bsimpl.
-    Unshelve. tea.
-    now bsimpl.
+    unshelve eapply WLRTmRedIrrelevant'.
+    5: unshelve eapply appTerm.
+    6-9: eauto.
+    1: eapply LogtoW.
+    1,2: now bsimpl.
   Qed.
 
-  Lemma arr_wk {Γ Δ A B} {ρ : Δ ≤ Γ} : arr A⟨ρ⟩ B⟨ρ⟩ = (arr A B)⟨ρ⟩.
-  Proof. cbn; now bsimpl. Qed.
+    
+  Lemma Wsimple_appTerm {wl Γ t u F G l}
+    {RF : W[Γ ||-<l> F]< wl >}
+    (RG : W[Γ ||-<l> G]< wl >) 
+    (RΠ : W[Γ ||-<l> arr F G]< wl >)
+    (Rt : W[Γ ||-<l> t : arr F G | RΠ]< wl >)
+    (Ru : W[Γ ||-<l> u : F | RF]< wl >) :
+    W[Γ ||-<l> tApp t u : G| RG]< wl >.
+  Proof.
+    unshelve eapply WLRTmRedIrrelevant'.
+    5: unshelve eapply WappTerm.
+    6-9: eauto.
+    1,2: now bsimpl.
+  Qed.
 
-  Lemma wkRedArr {Γ l A B f} 
-    (RA : [Γ ||-<l> A]) 
-    (RB : [Γ ||-<l> B]) 
-    {Δ} (ρ : Δ ≤ Γ) (wfΔ : [|- Δ]) :
-    [Γ ||-<l> f : arr A B | ArrRedTy RA RB] ->
-    [Δ ||-<l> f⟨ρ⟩ : arr A⟨ρ⟩ B⟨ρ⟩ | ArrRedTy (wk ρ wfΔ RA) (wk ρ wfΔ RB)].
+
+  Lemma simple_appcongTerm {wl Γ t t' u u' F G l}
+    {RF : [Γ ||-<l> F]< wl >}
+    (RG : [Γ ||-<l> G]< wl >)
+    (RΠ : [Γ ||-<l> arr F G]< wl >) 
+    (Rtt' : [Γ ||-<l> t ≅ t' : _ | RΠ]< wl >)
+    (Ru : [Γ ||-<l> u : F | RF]< wl >)
+    (Ru' : [Γ ||-<l> u' : F | RF]< wl >)
+    (Ruu' : [Γ ||-<l> u ≅ u' : F | RF ]< wl >) :
+      W[Γ ||-<l> tApp t u ≅ tApp t' u' : G | (LogtoW RG)]< wl >.
+  Proof.
+    unshelve eapply WLRTmEqIrrelevant'.
+    5: unshelve eapply appcongTerm.
+    7-12: tea.
+    1: eapply LogtoW.
+    1,2: now bsimpl.
+  Qed.
+    
+
+  Lemma Wsimple_appcongTerm {wl Γ t t' u u' F G l}
+    {RF : W[Γ ||-<l> F]< wl >}
+    (RG : W[Γ ||-<l> G]< wl >)
+    (RΠ : W[Γ ||-<l> arr F G]< wl >) 
+    (Rtt' : W[Γ ||-<l> t ≅ t' : _ | RΠ]< wl >)
+    (Ru : W[Γ ||-<l> u : F | RF]< wl >)
+    (Ru' : W[Γ ||-<l> u' : F | RF]< wl >)
+    (Ruu' : W[Γ ||-<l> u ≅ u' : F | RF ]< wl >) :
+      W[Γ ||-<l> tApp t u ≅ tApp t' u' : G | RG]< wl >.
+  Proof.
+    unshelve eapply WLRTmEqIrrelevant'.
+    5: unshelve eapply WappcongTerm.
+    7-12: tea.
+    1,2: now bsimpl.
+  Qed.
+
+  Lemma wkRedArr {wl Γ l A B f} 
+    (RA : [Γ ||-<l> A]< wl >) 
+    (RB : [Γ ||-<l> B]< wl >) 
+    {Δ} (ρ : Δ ≤ Γ) (wfΔ : [|- Δ]< wl >) :
+    [Γ ||-<l> f : arr A B | ArrRedTy RA RB]< wl > ->
+    [Δ ||-<l> f⟨ρ⟩ : arr A⟨ρ⟩ B⟨ρ⟩ | ArrRedTy (wk ρ wfΔ RA) (wk ρ wfΔ RB)]< wl >.
   Proof.
     intro; irrelevance0.
     2: unshelve eapply wkTerm; cycle 3; tea.
-    symmetry; apply arr_wk.
+    symmetry; apply wk_arr.
   Qed.
 
-  Lemma compred {Γ l A B C f g} 
-    (RA : [Γ ||-<l> A]) 
-    (RB : [Γ ||-<l> B]) 
-    (RC : [Γ ||-<l> C]) :
-    [Γ ||-<l> f : arr A B | ArrRedTy RA RB] ->
-    [Γ ||-<l> g : arr B C | ArrRedTy RB RC] ->
-    [Γ ||-<l> comp A g f : arr A C | ArrRedTy RA RC].
+  Definition compred_appTree {wl Γ l A B C f g} 
+    (RA : [Γ ||-<l> A]< wl >) 
+    (RB : [Γ ||-<l> B]< wl >) 
+    (RC : [Γ ||-<l> C]< wl >) :
+    [LRPi' (normRedΠ0 (invLRΠ (ArrRedTy RA RB))) | Γ ||- f : arr A B ]< wl > ->
+    [LRPi' (normRedΠ0 (invLRΠ (ArrRedTy RB RC))) | Γ ||- g : arr B C ]< wl > ->
+    forall Δ wl' a (ρ : Δ ≤ Γ) (tau : wl' ≤ε wl)
+                       (wfΔ : [|- Δ]< wl' >)
+                       (ha : [PolyRedPack.shpRed (normRedΠ0 (invLRΠ (ArrRedTy RA RB))) ρ tau wfΔ | Δ ||- a
+                               : (ParamRedTyPack.dom (normRedΠ0 (invLRΠ (ArrRedTy RA RB))))⟨ρ⟩ ]< wl' >),
+    DTree wl'.
   Proof.
-    intros Rf Rg.
-    normRedΠin ΠAB Rf; normRedΠin ΠBC Rg; normRedΠ ΠAC. 
-    assert (h : forall Δ a (ρ : Δ ≤ Γ) (wfΔ : [|- Δ]) RA (ha : [Δ ||-<l> a : A⟨ρ⟩ | RA]),
-      [Δ ||-<l> tApp g⟨ρ⟩ (tApp f⟨ρ⟩ a) : _ | wk ρ wfΔ RC]).
-    1:{
-      intros; eapply simple_appTerm; [|eapply simple_appTerm; tea].
-      1,2: eapply wkRedArr; irrelevance.
-      Unshelve. 1: eapply wk. all: tea.
-    }
-    assert (heq : forall Δ a b (ρ : Δ ≤ Γ) (wfΔ : [|- Δ]) RA
-      (ha : [Δ ||-<l> a : A⟨ρ⟩ | RA]) (hb : [Δ ||-<l> b : A⟨ρ⟩ | RA])
-      (ha : [Δ ||-<l> a ≅ b: A⟨ρ⟩ | RA]),
-      [Δ ||-<l> tApp g⟨ρ⟩ (tApp f⟨ρ⟩ a) ≅ tApp g⟨ρ⟩ (tApp f⟨ρ⟩ b) : _ | wk ρ wfΔ RC]).
+    intros Rf Rg * ha.
+    unshelve eapply DTree_bind_over.
+    - eapply DTree_fusion.
+      + now unshelve eapply (PiRedTm.appTree (a := a) Rf).
+      + now unshelve eapply (PolyRedPack.posTree (normRedΠ0 (invLRΠ (ArrRedTy RA RB)))).
+    - intros wl'' Hover.
+      pose proof (f' := over_tree_le Hover).
+      unshelve eapply (PiRedTm.appTree Rg).
+      3: eassumption.
+      2: now eapply wfLCon_le_trans.
+      2: now eapply wfc_Ltrans.
+      2: irrelevance0 ; [ | eapply (PiRedTm.app Rf)] .
+      2: eapply over_tree_fusion_l ; eassumption.
+      cbn.
+      bsimpl.
+      now rewrite rinstInst'_term.
+      Unshelve.
+      now eapply over_tree_fusion_r.
+  Defined.
+  
+  Lemma compred {wl Γ l A B C u v} 
+    (RA : [Γ ||-<l> A]< wl >) 
+    (RB : [Γ ||-<l> B]< wl >) 
+    (RC : [Γ ||-<l> C]< wl >) :
+    [Γ ||-<l> u : arr A B | ArrRedTy RA RB]< wl > ->
+    [Γ ||-<l> v : arr B C | ArrRedTy RB RC]< wl > ->
+    [Γ ||-<l> comp A v u : arr A C | ArrRedTy RA RC]< wl >.
+  Proof.
+    intros Ru Rv.
+    normRedΠin Ru; normRedΠin Rv; normRedΠ ΠAC.
+    pose (d := compred_appTree RA RB RC Ru Rv).
+    assert (h : forall Δ wl' a (ρ : Δ ≤ Γ) (f : wl' ≤ε wl)
+                       (wfΔ : [|- Δ]< wl' >) RA
+                       (ha : [Δ ||-<l> a : A⟨ρ⟩ | RA]< wl' >),
+               W[Δ ||-<l> tApp v⟨ρ⟩ (tApp u⟨ρ⟩ a) : _ | Wwk ρ wfΔ (WLtrans f (LogtoW RC))]< wl' >).
     1:{
       intros.
-      eapply simple_appcongTerm; [| | |eapply simple_appcongTerm; tea].
-      1,4: eapply LREqTermRefl_; eapply wkRedArr; irrelevance.
-      1,2: eapply simple_appTerm; tea; eapply wkRedArr; irrelevance.
-      Unshelve. 1: eapply wk. all: tea.
+      eapply WLRTmRedIrrelevant' ; [reflexivity | ].
+      unshelve eapply Wsimple_appTerm.
+      5: eapply simple_appTerm.
+      3: eapply TmLogtoW.
+      2,3: eapply wkRedArr.
+      1,2: irrelevance0 ; [reflexivity | ].
+      1,2: eapply (Tm_Ltrans f) ; eassumption.
+      eassumption.
+      Unshelve.
+      3,6: eassumption.
+      1: eapply LogtoW.
+      1,2: eapply wk ; try eassumption.
+      all: now eapply (Ltrans f).
+    }
+    assert (heq : forall Δ wl' a b (ρ : Δ ≤ Γ) (f : wl' ≤ε wl)
+                         (wfΔ : [|- Δ]< wl' >) RA
+                         (ha : [Δ ||-<l> a : A⟨ρ⟩ | RA]< wl' >)
+                         (hb : [Δ ||-<l> b : A⟨ρ⟩ | RA]< wl' >)
+                         (hab : [Δ ||-<l> a ≅ b: A⟨ρ⟩ | RA]< wl' >),
+               W[Δ ||-<l> tApp v⟨ρ⟩ (tApp u⟨ρ⟩ a) ≅ tApp v⟨ρ⟩ (tApp u⟨ρ⟩ b) : _ |
+                  Wwk ρ wfΔ (WLtrans f (LogtoW RC))]< wl' >).
+    1:{
+      intros.
+      eapply WLRTmEqIrrelevant' ; [reflexivity | ].
+      eapply Wsimple_appcongTerm ; [| | | unshelve eapply simple_appcongTerm ].
+      1: eapply TmEqLogtoW.
+      1,8: unshelve eapply reflLRTmEq, wkRedArr, (Tm_Ltrans' f).
+      2,7,11,12,17-19: eassumption.
+      1-4: now eapply (Ltrans f).
+      1,2: unshelve eapply simple_appTerm.
+      7,9: unshelve eapply wkRedArr, (Tm_Ltrans' f).
+      13,14: irrelevance.
+      6,10: now eapply ArrRedTy.
+      all: try eassumption.
+      5: eapply wk ; eauto.
+      all: now eapply (Ltrans f).
+      Unshelve.
+      now eapply LogtoW, wk, (Ltrans f).
     }
     escape.
-    assert (beta : forall Δ a (ρ : Δ ≤ Γ) (wfΔ : [|- Δ]) RA (ha : [Δ ||-<l> a : A⟨ρ⟩ | RA]),
-      [Δ ||-<l> tApp (comp A g f)⟨ρ⟩ a : _ | wk ρ wfΔ RC] ×
-      [Δ ||-<l> tApp (comp A g f)⟨ρ⟩ a ≅ tApp g⟨ρ⟩ (tApp f⟨ρ⟩ a) : _ | wk ρ wfΔ RC]).
+    assert (beta : forall Δ wl' a (ρ : Δ ≤ Γ) (f : wl' ≤ε wl)
+                          (wfΔ : [|- Δ]< wl' >) RA
+                          (ha : [Δ ||-<l> a : A⟨ρ⟩ | RA]< wl' >),
+               W[Δ ||-<l> tApp (comp A v u)⟨ρ⟩ a : _ | Wwk ρ wfΔ (WLtrans f (LogtoW RC))]< wl' > ×
+               W[Δ ||-<l> tApp (comp A v u)⟨ρ⟩ a ≅ tApp v⟨ρ⟩ (tApp u⟨ρ⟩ a) : _ |
+                  Wwk ρ wfΔ (WLtrans f (LogtoW RC))]< wl' >).
     1:{
       intros; cbn. 
       assert (eq : forall t : term, t⟨↑⟩⟨upRen_term_term ρ⟩ = t⟨ρ⟩⟨↑⟩) by (intros; now asimpl).
       do 2 rewrite eq.
-      eapply redSubstTerm.
+      eapply WredSubstTerm.
       + now eapply h.
       + eapply redtm_comp_beta.
         6: cbn in *; now escape.
-        5: erewrite arr_wk; eapply ty_wk; tea.
+        5: now erewrite wk_arr; eapply ty_wk, ty_Ltrans; tea.
         4: eapply typing_meta_conv.
-        4: eapply ty_wk; tea.
-        4: now rewrite <- arr_wk.
-        1-3: now eapply wft_wk.
+        4: now eapply ty_wk, ty_Ltrans; tea.
+        4: exact (wk_arr (A := A) (B := B) ρ).
+        1-3: now eapply wft_wk, wft_Ltrans.
     }
     econstructor.
     - eapply redtmwf_refl.
-      eapply ty_comp; cycle 2; tea.
-    - constructor.
-    - apply tm_nf_lam.
-      + now eapply reifyType.
-      + change (PiRedTy.dom (PiRedTyPack.toPiRedTy ΠAC)) with A.
-        change (PiRedTy.cod (PiRedTyPack.toPiRedTy ΠAC)) with C⟨↑⟩.
-        pose (ρ := @wk_step Γ Γ A wk_id).
-        assert (Hr : forall (t : term), t⟨↑⟩ = t⟨ρ⟩).
-        { unfold ρ; bsimpl; reflexivity. }
-        do 3 rewrite Hr.
-        eapply reifyTerm.
-        unshelve refine (h _ (tRel 0) ρ _ (wk _ _ RA) _).
-        1,2: gen_typing.
-        apply var0; [|tea]; unfold ρ; bsimpl; reflexivity.
-    - cbn. eapply convtm_comp; cycle 3; tea.
+      eapply ty_comp ; cycle 2 ; now tea.
+    - cbn. eapply convtm_comp; cycle 6; tea.
       erewrite <- wk1_ren_on.
-      eapply escapeEqTerm.
-      eapply LREqTermRefl_.
+      eapply WescapeEqTerm.
+      eapply WreflLRTmEq.
       do 2 erewrite <- wk1_ren_on.
       eapply h.
       eapply var0; now bsimpl.
-      Unshelve. 1: gen_typing.
-      eapply wk; tea; gen_typing.
-    - intros; cbn.
+      { now eapply wfc_ty. }
+      unshelve eapply escapeEq, reflLRTyEq; tea.
+      unshelve eapply escapeEq, reflLRTyEq; tea.
+      Unshelve. 3: gen_typing.
+      3: now eapply wfLCon_le_id.
+      3: now eapply wk; tea; gen_typing.
+      1:{ intros ; eapply DTree_fusion.
+          + now unshelve eapply (fst (beta _ _ _ _ _ Hd _ ha)).
+          + unshelve eapply (WTTmEq (Wwk ρ Hd (WLtrans f (LogtoW RC))) _).
+            3: now unshelve eapply (snd (beta _ _ _ _ _ _ _ ha)).
+      }
+      intros ; eapply DTree_fusion.
+      + now unshelve eapply (WTTmEq _ (heq _ _ _ _ _ _ Hd _ ha hb eq)).
+      + exact (WT C⟨ρ⟩ (Wwk ρ Hd (WLtrans f (LogtoW RC)))).
+    - unshelve econstructor 1; intros; cbn.
+      + eapply h ; eassumption.
+      + apply reflLRTyEq.
+      + assert (Hrw : forall t, t⟨↑⟩[a .: ρ >> tRel] = t⟨ρ⟩).
+        { intros; bsimpl; symmetry; now apply rinstInst'_term. }
+        do 2 rewrite Hrw; irrelevance0; [symmetry; apply Hrw|].
+        unshelve eapply h.
+        7: exact Ho'.
+        cbn ; now eapply over_tree_le.
+    - intros; cbn in *.
       irrelevance0.
-      2: unshelve eapply beta; tea.
-      bsimpl; now rewrite rinstInst'_term.
-    - intros; irrelevance0; cycle 1.
+      2: unshelve eapply (fst (beta _ _ _ _ _ _ _ _)) ; cbn.
+      3,4,6: eassumption.
+      + bsimpl; now rewrite rinstInst'_term.
+      + now eapply over_tree_le.
+      + now eapply over_tree_fusion_l.
+    - intros * hb hab ** ; irrelevance0; cycle 1 ; cbn in *.
       1: eapply transEqTerm;[|eapply transEqTerm].
-      + unshelve eapply beta; tea.
-      + unshelve eapply heq; tea.
-      + eapply LRTmEqSym.
-        unshelve eapply beta; tea.
-      + cbn; bsimpl; now rewrite rinstInst'_term.
-  Qed. 
+      1:{ unshelve eapply (snd (beta _ _ _ _ _ _ _ _)) ; cbn in *.
+          2,3,5: eassumption.
+          * now eapply over_tree_le.
+          * now eapply over_tree_fusion_r.
+      }
+      2:{ eapply LRTmEqSym.
+          unshelve eapply  (snd (beta _ _ _ _ _ _ _ _)).
+          2: eassumption.
+          cbn in *.
+          eapply over_tree_fusion_r ; eassumption.
+      }
+      cbn in *.
+      irrelevance0 ; [ reflexivity | ].
+      2: cbn ;  bsimpl ; now rewrite rinstInst'_term.
+      unshelve eapply heq.
+      2,3,6-8: eassumption.
+      + now eapply over_tree_fusion_r.
+      + now eapply over_tree_fusion_l.
+  Qed.
 
 End SimpleArrow.
